template-coq/theories/WcbvEval.v
@@ -145,7 +145,7 @@ Section Wcbv.
       eval discr (mkApps (tConstruct ci.(ci_ind) c u) args) ->
       nth_error brs c = Some br ->
       declared_constructor Σ (ci.(ci_ind), c) mdecl idecl cdecl ->
-      let bctx := case_branch_context p cdecl in
+      let bctx := case_branch_context ci.(ci_ind) mdecl cdecl p br in
       #|skipn (ci_npar ci) args| = context_assumptions bctx ->
       eval (iota_red ci.(ci_npar) args bctx br) res ->
       eval (tCase ci p discr brs) res
@@ -231,7 +231,7 @@ Section Wcbv.
           P discr (mkApps (tConstruct ind c u) args) ->
           nth_error brs c = Some br ->
           declared_constructor Σ (ci.(ci_ind), c) mdecl idecl cdecl ->
-          let bctx := case_branch_context p cdecl in
+          let bctx := case_branch_context ci.(ci_ind) mdecl cdecl p br in
           #|skipn (ci_npar ci) args| = context_assumptions bctx ->
           eval (iota_red npar args bctx br) res -> P (iota_red npar args bctx br) res -> 
           P (tCase ci p discr brs) res) ->
