template-coq/theories/utils/MCProd.v
@@ -72,3 +72,40 @@ Qed.
 
 Definition swap {A B : Type} (x : A * B) : B * A :=
   (snd x, fst x).
+
+(** n-ary cartesian products in Type, for shorter and more readable intro-patterns *)
+
+Reserved Notation "[ × P1 & P2 ]" (at level 0).
+Reserved Notation "[ × P1 , P2 & P3 ]" (at level 0, format
+  "'[hv' [ × '['  P1 , '/'  P2 ']' '/ '  &  P3 ] ']'").
+Reserved Notation "[ × P1 , P2 , P3 & P4 ]" (at level 0, format
+  "'[hv' [ × '['  P1 , '/'  P2 , '/'  P3 ']' '/ '  &  P4 ] ']'").
+Reserved Notation "[ × P1 , P2 , P3 , P4 & P5 ]" (at level 0, format
+  "'[hv' [ × '['  P1 , '/'  P2 , '/'  P3 , '/'  P4 ']' '/ '  &  P5 ] ']'").
+Reserved Notation "[ × P1 , P2 , P3 , P4 , P5 & P6 ]" (at level 0, format
+  "'[hv' [ × '['  P1 , '/'  P2 , '/'  P3 , '/'  P4 , '/'  P5 ']' '/ '  &  P6 ] ']'").
+Reserved Notation "[ × P1 , P2 , P3 , P4 , P5 , P6 & P7 ]" (at level 0, format
+"'[hv' [ × '['  P1 , '/'  P2 , '/'  P3 , '/'  P4 , '/'  P5 , '/'  P6  ']' '/ '  &  P7 ] ']'").
+Reserved Notation "[ × P1 , P2 , P3 , P4 , P5 , P6 , P7 & P8 ]" (at level 0, format
+"'[hv' [ × '['  P1 , '/'  P2 , '/'  P3 , '/'  P4 , '/'  P5 , '/'  P6 , '/'  P7 ']' '/ '  &  P8 ] ']'").
+Reserved Notation "[ × P1 , P2 , P3 , P4 , P5 , P6 , P7 , P8 & P9 ]" (at level 0, format
+"'[hv' [ × '['  P1 , '/'  P2 , '/'  P3 , '/'  P4 , '/'  P5 , '/'  P6 , '/'  P7 , '/'  P8 ']' '/ '  &  P9 ] ']'").
+
+Variant and3 (P1 P2 P3 : Type) : Type := Times3 of P1 & P2 & P3.
+Variant and4 (P1 P2 P3 P4 : Type) : Type := Times4 of P1 & P2 & P3 & P4.
+Variant and5 (P1 P2 P3 P4 P5 : Type) : Type := Times5 of P1 & P2 & P3 & P4 & P5.
+Variant and6 (P1 P2 P3 P4 P5 P6 : Type) : Type := Times6 of P1 & P2 & P3 & P4 & P5 & P6.
+Variant and7 (P1 P2 P3 P4 P5 P6 P7 : Type) : Type := Times7 of P1 & P2 & P3 & P4 & P5 & P6 & P7.
+Variant and8 (P1 P2 P3 P4 P5 P6 P7 P8 : Type) : Type := Times8 of P1 & P2 & P3 & P4 & P5 & P6 & P7 & P8.
+Variant and9 (P1 P2 P3 P4 P5 P6 P7 P8 P9 : Type) : Type := Times9 of P1 & P2 & P3 & P4 & P5 & P6 & P7 & P8 & P9.
+
+Hint Constructors and3 and3 and5 and6 : core.
+
+Notation "[ × P1 & P2 ]" := (pair P1 P2) (only parsing) : type_scope.
+Notation "[ × P1 , P2 & P3 ]" := (and3 P1 P2 P3) : type_scope.
+Notation "[ × P1 , P2 , P3 & P4 ]" := (and4 P1 P2 P3 P4) : type_scope.
+Notation "[ × P1 , P2 , P3 , P4 & P5 ]" := (and5 P1 P2 P3 P4 P5) : type_scope.
+Notation "[ × P1 , P2 , P3 , P4 , P5 & P6 ]" := (and6 P1 P2 P3 P4 P5 P6) : type_scope.
+Notation "[ × P1 , P2 , P3 , P4 , P5 , P6 & P7 ]" := (and7 P1 P2 P3 P4 P5 P6 P7) : type_scope.
+Notation "[ × P1 , P2 , P3 , P4 , P5 , P6 , P7 & P8 ]" := (and8 P1 P2 P3 P4 P5 P6 P7 P8) : type_scope.
+Notation "[ × P1 , P2 , P3 , P4 , P5 , P6 , P7 , P8 & P9 ]" := (and9 P1 P2 P3 P4 P5 P6 P7 P8 P9) : type_scope.
